theories/seq_product.v
@@ -1,5 +1,6 @@
 Require Export refframe.module.
 Require Import refframe.trefines.
+Require Import refframe.proof_techniques.
 
 (*** [seq_product] *)
 Inductive seq_product_state :=
@@ -35,6 +36,7 @@ Inductive seq_product_step {EV1 EV2} (m1 : module EV1) (m2 : module EV2) :
 
 Definition mod_seq_product {EV1 EV2} (m1 : module EV1) (m2 : module EV2) : module (seq_product_event EV1 EV2) :=
   Mod (seq_product_step m1 m2).
+Global Hint Transparent mod_seq_product : tstep.
 
 Global Instance seq_product_vis_no_all {EV1 EV2} (m1 : module EV1) (m2 : module EV2) `{!VisNoAll m1} `{!VisNoAll m2}:
   VisNoAll (mod_seq_product m1 m2).
@@ -268,3 +270,40 @@ Proof.
   move => [/=Hr1] [/=Hr2]. constructor => κs /= /seq_product_to_mods[κs1 [κs2 [/Hr1 ? /Hr2 ?]]].
   by apply: mods_to_seq_product.
 Qed.
+
+(** * tstep *)
+Lemma mod_seq_product_step_None_i {EV1 EV2} (m1 : module EV1) (m2 : module EV2) σ1 σ2:
+  TStepI (mod_seq_product m1 m2) (SPNone, σ1, σ2) (λ G, ∀ s, G true (Some (SPENone s)) (λ G', G' (s, σ1, σ2))).
+Proof.
+  constructor => G HG. apply: TDStep => ???. invert_all @m_step. left.
+  eexists _. split; [done|]. naive_solver.
+Qed.
+Global Hint Resolve mod_seq_product_step_None_i : tstep.
+
+Lemma mod_seq_product_step_l_i {EV1 EV2} (m1 : module EV1) (m2 : module EV2) σ1 σ2 P `{!TStepI m1 σ1 P}:
+  TStepI (mod_seq_product m1 m2) (SPLeft, σ1, σ2) (λ G, P (λ b κ G',
+    ∀ s', (if κ is None then s' = SPLeft else True) →
+     G b ((λ e, SPELeft e s') <$> κ) (λ Pσ, G' (λ x, Pσ (s', x, σ2))))).
+Proof.
+  constructor => G /tstepi_proof HP.
+  apply: (thas_trace_dual_submodule _ (mod_seq_product _ _) (λ x, (SPLeft, x, σ2))); [done| |].
+  - move => ?? /= [?[HG HG']]. eexists _. split; [by apply HG|] => ? /= /HG'[?[??]]. naive_solver.
+  - move => ????. invert_all' @m_step; simplify_eq/=; eexists _, _.
+    split_and!; [done| |naive_solver].
+    move => [?[HG HG']]. eexists _. split; [by apply HG|] => ? /= /HG'[?[??]]. naive_solver.
+Qed.
+Global Hint Resolve mod_seq_product_step_l_i : tstep.
+
+Lemma mod_seq_product_step_r_i {EV1 EV2} (m1 : module EV1) (m2 : module EV2) σ1 σ2 P `{!TStepI m2 σ2 P}:
+  TStepI (mod_seq_product m1 m2) (SPRight, σ1, σ2) (λ G, P (λ b κ G',
+    ∀ s', (if κ is None then s' = SPRight else True) →
+     G b ((λ e, SPERight e s') <$> κ) (λ Pσ, G' (λ x, Pσ (s', σ1, x))))).
+Proof.
+  constructor => G /tstepi_proof HP.
+  apply: (thas_trace_dual_submodule _ (mod_seq_product _ _) (λ x, (SPRight, σ1, x))); [done| |].
+  - move => ?? /= [?[HG HG']]. eexists _. split; [by apply HG|] => ? /= /HG'[?[??]]. naive_solver.
+  - move => ????. invert_all' @m_step; simplify_eq/=; eexists _, _.
+    split_and!; [done| |naive_solver].
+    move => [?[HG HG']]. eexists _. split; [by apply HG|] => ? /= /HG'[?[??]]. naive_solver.
+Qed.
+Global Hint Resolve mod_seq_product_step_r_i : tstep.
