theories/itree.v
@@ -357,43 +357,44 @@ Qed.
 (** These step rules should always apply to itree with a bind at the
 top-level and discriminate on the argument of the bind.
 TODO: add a step rule that adds a bind a the top-level if there is none.  *)
-Lemma itree_step_bind_s EV S A B (t : itree _ A) (k : A → itree _ B) h s κs:
-  TStepS (mod_itree EV S) (ITree.bind (ITree.bind t k) h, s) κs
-            (λ G, itree_rel (G κs) ((ITree.bind t (fun r => ITree.bind (k r) h)), s)).
+Lemma itree_step_bind_s EV S A B (t : itree _ A) (k : A → itree _ B) h s:
+  TStepS (mod_itree EV S) (ITree.bind (ITree.bind t k) h, s)
+            (λ κs G, itree_rel (G κs) ((ITree.bind t (fun r => ITree.bind (k r) h)), s)).
 Proof.
-  constructor => G HG. eexists tnil, _. split; [simpl; done|].
+  constructor => κs G HG. eexists tnil, _. split; [simpl; done|].
   apply itree_rel_intro. rewrite bind_bind. tend.
 Qed.
 Global Hint Resolve itree_step_bind_s : tstep.
 
-Lemma itree_step_Ret_s EV S A (x : A) h s κs:
-  TStepS (mod_itree EV S) (ITree.bind (Ret x) h, s) κs (λ G, itree_rel (G κs) (h x, s)).
+Lemma itree_step_Ret_s EV S A (x : A) h s:
+  TStepS (mod_itree EV S) (ITree.bind (Ret x) h, s) (λ κs G, itree_rel (G κs) (h x, s)).
 Proof.
   constructor => ?. eexists tnil, _. split; [simpl; done|].
   apply itree_rel_intro. rewrite bind_ret_l. tend.
 Qed.
 Global Hint Resolve itree_step_Ret_s : tstep.
 
-Lemma itree_step_Tau_s EV S t s κs:
-  TStepS (mod_itree EV S) (Tau t, s) κs (λ G, itree_rel (G κs) (t, s)).
+Lemma itree_step_Tau_s EV S t s:
+  TStepS (mod_itree EV S) (Tau t, s) (λ κs G, itree_rel (G κs) (t, s)).
 Proof.
   constructor => ?. eexists tnil, _. split; [simpl; done|].
   apply itree_rel_intro. rewrite tau_eutt. tend.
 Qed.
 Global Hint Resolve itree_step_Tau_s : tstep.
 
-Lemma itree_step_Vis_s EV S k s κs e e':
-  TStepS (mod_itree EV S) (TVis e;;;; k, s) (tcons e' κs) (λ G, e = e' ∧ itree_rel (G κs) (k, s)).
+Lemma itree_step_Vis_s EV S k s e:
+  TStepS (mod_itree EV S) (TVis e;;;; k, s) (λ κs G,
+    if κs is tcons e' κs' then e = e' ∧ itree_rel (G κs') (k, s) else False).
 Proof.
-  constructor => ?[??]. subst. eexists (tcons e' tnil), _. split; [simpl; done|].
+  constructor => ??. case_match => // -[??]. subst. eexists (tcons _ tnil), _. split; [simpl; done|].
   apply itree_rel_intro. rewrite bind_trigger.
   apply: thas_trace_Vis. tend.
 Qed.
 Global Hint Resolve itree_step_Vis_s : tstep.
 
-Lemma itree_step_All_s EV S T k s κs:
-  TStepS (mod_itree EV S) (x ← TAll T;;; k x, s) κs
-            (λ G, ∀ x, itree_rel (G κs) (k x, s)).
+Lemma itree_step_All_s EV S T k s:
+  TStepS (mod_itree EV S) (x ← TAll T;;; k x, s)
+            (λ κs G, ∀ x, itree_rel (G κs) (k x, s)).
 Proof.
   constructor => ?. eexists tnil, _. split; [simpl; done|].
   apply itree_rel_intro. rewrite bind_trigger.
@@ -401,27 +402,27 @@ Proof.
 Qed.
 Global Hint Resolve itree_step_All_s : tstep.
 
-Lemma itree_step_Exist_s EV S T k s κs:
-  TStepS (mod_itree EV S) (x ← TExist T;;; k x, s) κs
-            (λ G, ∃ x, itree_rel (G κs) (k x, s)).
+Lemma itree_step_Exist_s EV S T k s:
+  TStepS (mod_itree EV S) (x ← TExist T;;; k x, s)
+            (λ κs G, ∃ x, itree_rel (G κs) (k x, s)).
 Proof.
-  constructor => ? [??]. eexists tnil, _. split; [simpl; done|].
+  constructor => ??[??]. eexists tnil, _. split; [simpl; done|].
   apply itree_rel_intro. rewrite bind_trigger.
   apply: thas_trace_Exist. tend.
 Qed.
 Global Hint Resolve itree_step_Exist_s : tstep.
 
-Lemma itree_step_Ub_s EV S T (k : T → _) s κs:
-  TStepS (mod_itree EV S) (x ← TUb;;; k x, s) κs (λ G, True).
+Lemma itree_step_Ub_s EV S T (k : T → _) s:
+  TStepS (mod_itree EV S) (x ← TUb;;; k x, s) (λ _ G, True).
 Proof.
-  constructor => ??. eexists tnil, _. split; [simpl; done|].
+  constructor => ???. eexists tnil, _. split; [simpl; done|].
   apply itree_rel_intro. rewrite /TUb bind_bind bind_trigger.
   apply: thas_trace_All. case.
 Qed.
 Global Hint Resolve itree_step_Ub_s : tstep.
 
-Lemma itree_step_Assume_s EV S P k s κs:
-  TStepS (mod_itree EV S) (TAssume P;;;; k, s) κs (λ G, P → itree_rel (G κs) (k, s)).
+Lemma itree_step_Assume_s EV S P k s:
+  TStepS (mod_itree EV S) (TAssume P;;;; k, s) (λ κs G, P → itree_rel (G κs) (k, s)).
 Proof.
   constructor => ??. eexists tnil, _. split; [simpl; done|].
   apply itree_rel_intro. rewrite /TAssume bind_bind bind_trigger.
@@ -429,17 +430,17 @@ Proof.
 Qed.
 Global Hint Resolve itree_step_Assume_s : tstep.
 
-Lemma itree_step_Assert_s EV S P k s κs:
-  TStepS (mod_itree EV S) (TAssert P;;;; k, s) κs (λ G, P ∧ itree_rel (G κs) (k, s)).
+Lemma itree_step_Assert_s EV S P k s:
+  TStepS (mod_itree EV S) (TAssert P;;;; k, s) (λ κs G, P ∧ itree_rel (G κs) (k, s)).
 Proof.
-  constructor => ? [??]. eexists tnil, _. split; [simpl; done|].
+  constructor => ?? [??]. eexists tnil, _. split; [simpl; done|].
   apply itree_rel_intro. rewrite /TAssert bind_bind bind_trigger.
   apply: thas_trace_Exist. { by constructor. } rewrite bind_ret_l. tend.
 Qed.
 Global Hint Resolve itree_step_Assert_s : tstep.
 
-Lemma itree_step_AssumeOpt_s EV S A (o : option A) k s κs:
-  TStepS (mod_itree EV S) (x ← TAssumeOpt o;;; k x, s) κs (λ G, ∀ x, (o = Some x) → itree_rel (G κs) (k x, s)).
+Lemma itree_step_AssumeOpt_s EV S A (o : option A) k s:
+  TStepS (mod_itree EV S) (x ← TAssumeOpt o;;; k x, s) (λ κs G, ∀ x, (o = Some x) → itree_rel (G κs) (k x, s)).
 Proof.
   constructor => ??. eexists tnil, _. split; [simpl; done|].
   apply itree_rel_intro. rewrite /TAssume bind_bind bind_trigger.
@@ -447,18 +448,18 @@ Proof.
 Qed.
 Global Hint Resolve itree_step_AssumeOpt_s : tstep.
 
-Lemma itree_step_AssertOpt_s EV S A (o : option A) k s κs:
-  TStepS (mod_itree EV S) (x ← TAssertOpt o;;; k x, s) κs (λ G, ∃ x, o = Some x ∧ itree_rel (G κs) (k x, s)).
+Lemma itree_step_AssertOpt_s EV S A (o : option A) k s:
+  TStepS (mod_itree EV S) (x ← TAssertOpt o;;; k x, s) (λ κs G, ∃ x, o = Some x ∧ itree_rel (G κs) (k x, s)).
 Proof.
-  constructor => ? [?[??]]. subst. eexists tnil, _. split; [simpl; done|].
+  constructor => ?? [?[??]]. subst. eexists tnil, _. split; [simpl; done|].
   apply itree_rel_intro. rewrite /TAssert bind_bind bind_trigger.
   apply: (thas_trace_Exist _ (exist _ _ _)); [done|] => ?. rewrite bind_ret_l. tend.
 Qed.
 Global Hint Resolve itree_step_AssertOpt_s : tstep.
 
-Lemma itree_step_recursive_bind_translate_s EV S R Q A B (f : A → itree (callE A B +' _) _) (t : itree (moduleE EV S) R) (k : R → itree (_ +' moduleE EV S) Q) h s κs:
-  TStepS (mod_itree EV S) (x ← interp (recursive f) (ITree.bind (translate inr_ t) k);;; h x, s) κs
-            (λ G, itree_rel (G κs) ((ITree.bind t (fun r => x ← interp (recursive f) (k r);;; h x)), s)).
+Lemma itree_step_recursive_bind_translate_s EV S R Q A B (f : A → itree (callE A B +' _) _) (t : itree (moduleE EV S) R) (k : R → itree (_ +' moduleE EV S) Q) h s:
+  TStepS (mod_itree EV S) (x ← interp (recursive f) (ITree.bind (translate inr_ t) k);;; h x, s)
+            (λ κs G, itree_rel (G κs) ((ITree.bind t (fun r => x ← interp (recursive f) (k r);;; h x)), s)).
 Proof.
   constructor => ??. eexists tnil, _. split; [simpl; done|].
   apply itree_rel_intro. rewrite interp_bind bind_bind interp_translate /= interp_trigger_h.
@@ -466,18 +467,18 @@ Proof.
 Qed.
 Global Hint Resolve itree_step_recursive_bind_translate_s : tstep.
 
-Lemma itree_step_recursive_translate_s EV S R A B (f : A → itree (callE A B +' _) _) (t : itree (moduleE EV S) R) h s κs:
-  TStepS (mod_itree EV S) (x ← interp (recursive f) (translate inr_ t);;; h x, s) κs
-            (λ G, itree_rel (G κs) ((x ← t;;; h x), s)).
+Lemma itree_step_recursive_translate_s EV S R A B (f : A → itree (callE A B +' _) _) (t : itree (moduleE EV S) R) h s:
+  TStepS (mod_itree EV S) (x ← interp (recursive f) (translate inr_ t);;; h x, s)
+            (λ κs G, itree_rel (G κs) ((x ← t;;; h x), s)).
 Proof.
   constructor => ??. eexists tnil, _. split; [simpl; done|].
   apply itree_rel_intro. rewrite interp_translate /= interp_trigger_h.
   tend.
 Qed.
 Global Hint Resolve itree_step_recursive_translate_s : tstep.
-Lemma itree_step_recursive_call_s EV S R A B (f : A → itree (callE A B +' _) _) k (h : R → _) s κs a:
-  TStepS (mod_itree EV S) (x ← interp (recursive f) (y ← call a;;; k y);;; h x, s) κs
-            (λ G, itree_rel (G κs) ((y ← rec f a;;; x ← interp (recursive f) (k y);;; h x), s)).
+Lemma itree_step_recursive_call_s EV S R A B (f : A → itree (callE A B +' _) _) k (h : R → _) s a:
+  TStepS (mod_itree EV S) (x ← interp (recursive f) (y ← call a;;; k y);;; h x, s)
+            (λ κs G, itree_rel (G κs) ((y ← rec f a;;; x ← interp (recursive f) (k y);;; h x), s)).
 Proof.
   constructor => ??. eexists tnil, _. split; [simpl; done|].
   apply itree_rel_intro. rewrite interp_bind interp_recursive_call bind_bind.
@@ -485,8 +486,8 @@ Proof.
 Qed.
 Global Hint Resolve itree_step_recursive_call_s : tstep.
 
-Lemma itree_step_interp_ret_s EV S R E  (f : E ~> itree (moduleE EV S)) (a : R) h s κs:
-  TStepS (mod_itree EV S) (x ← interp f (Ret a);;; h x, s) κs (λ G, itree_rel (G κs) (h a, s)).
+Lemma itree_step_interp_ret_s EV S R E  (f : E ~> itree (moduleE EV S)) (a : R) h s:
+  TStepS (mod_itree EV S) (x ← interp f (Ret a);;; h x, s) (λ κs G, itree_rel (G κs) (h a, s)).
 Proof.
   constructor => ??. eexists tnil, _. split; [simpl; done|].
   apply itree_rel_intro. rewrite interp_ret bind_ret_l. tend.
